Introduce the TermRel constructive relation

Solver/Expr.v
@@ -51,16 +51,31 @@ Derive NoConfusion NoConfusionHom Subterm EqDec for positive STerm.
 Inductive Term {a o} (tys : Vector.t (obj_pair o) a) :
   obj_idx o → obj_idx o → Type :=
   | Ident {dom} : Term tys dom dom
-  | Morph (f : arr_idx a) : Term tys (fst (tys[@f])) (snd (tys[@f]))
+  | Morph (f : arr_idx a) :
+    Term tys (fst (tys[@f])) (snd (tys[@f]))
   | Comp {dom mid cod : obj_idx o}
          (f : Term tys mid cod) (g : Term tys dom mid) :
-      Term tys dom cod.
+    Term tys dom cod.
 
 Derive Signature NoConfusion for Term.
 
 Arguments Ident {a o tys dom}.
 Arguments Morph {a o tys} f.
 Arguments Comp {a o tys dom mid cod} f g.
+
+Inductive TermRel {a o} (tys : Vector.t (obj_pair o) a) :
+  STerm → ∀ {dom cod : obj_idx o}, Term tys dom cod → Type :=
+  | IsIdent {dom} : TermRel tys SIdent (Ident (dom:=dom))
+  | IsMorph (f : arr_idx a) :
+    @TermRel _ _ tys (SMorph (Fin_to_pos f))
+       (fst (tys[@f])) (snd (tys[@f])) (Morph f)
+  | IsComp {dom mid cod : obj_idx o} {sf sg}
+      (f : Term tys mid cod) (g : Term tys dom mid) :
+    TermRel tys sf f →
+    TermRel tys sg g →
+    TermRel tys (SComp sf sg) (Comp f g).
+
+Derive Signature for TermRel.
 
 Inductive SExpr : Set :=
   | STop
